some more top-down work on stabilization

systems/TreeAggregationDynamicLabeledCorrect.v
@@ -25,22 +25,28 @@ Require Import mathcomp.fingroup.fingroup.
 
 Require Import commfingroup.
 
+Require Import AAC_tactics.AAC.
+
+Set Bullet Behavior "Strict Subproofs".
+
 Local Arguments update {_} {_} _ _ _ _ _ : simpl never.
 
 Set Implicit Arguments.
 
 Module TreeAggregationCorrect (Import NT : NameType)
- (NOT : NameOrderedType NT) (NSet : MSetInterface.S with Module E := NOT) 
- (NOTC : NameOrderedTypeCompat NT) (NMap : FMapInterface.S with Module E := NOTC) 
- (Import RNT : RootNameType NT) 
+ (NOT : NameOrderedType NT) (NSet : MSetInterface.S with Module E := NOT)
+ (NOTC : NameOrderedTypeCompat NT) (NMap : FMapInterface.S with Module E := NOTC)
+ (Import RNT : RootNameType NT)
  (Import CFG : CommutativeFinGroup)
- (Import ANT : AdjacentNameType NT) 
+ (Import ANT : AdjacentNameType NT)
  (Import TA : TAux NT NOT NSet NOTC NMap)
  (Import AD : ADefs NT NOT NSet NOTC NMap CFG).
 
 Module TG := TreeAggregation NT NOT NSet NOTC NMap RNT CFG ANT TA AD.
-
 Import TG.
+
+Module ADCFGAACInstances := CFGAACInstances CFG.
+Import ADCFGAACInstances.
 
 Definition node_aggregate (state : name -> option data) (n : name) :=
   match state n with
@@ -60,7 +66,15 @@ Instance AggregationData_Data : AggregationData Data :=
     aggr_balance := balance
   }.
 
-Definition sum_local_nodes (net : ordered_dynamic_network) (nodes : list Net.name) : m :=
+Instance AggregationMsg_TreeAggregation : AggregationMsg :=
+  {
+    aggr_msg := msg ;
+    aggr_msg_eq_dec := msg_eq_dec ;
+    aggr_fail := Fail ;
+    aggr_of := fun mg => match mg with | Aggregate m' => m' | _ => 1%g end
+  }.
+
+Definition sum_local_nodes (net : ordered_dynamic_network) (nodes : list name) : m :=
   sum_local (filterMap net.(odnwState) nodes).
 
 Definition aggregation_msg (m : Msg) : bool :=
@@ -100,26 +114,143 @@ Lemma leaf_nodes_eventually_have_unit :
     event_step_star step_ordered_dynamic_failure step_ordered_dynamic_failure_init (hd s) ->
     leaf_node (snd (hd s).(evt_a)) failed n d ->
     lb_step_execution lb_step_ordered_dynamic_failure s ->
-    eventually (always (now (fun e =>
-                               exists d,
-                                 (snd e.(evt_a)).(odnwState) n = Some d /\
-                                 aggregate d = 1%g))) s.
+    continuously (now (fun e =>
+                         exists d,
+                           (snd e.(evt_a)).(odnwState) n = Some d /\
+                           aggregate d = 1%g)) s.
 Proof.
 Admitted.
 
-Theorem churn_free_stabilization : 
+Definition non_root_nodes_have_unit
+           (failed : list name)
+           (e : event (list name * ordered_dynamic_network)
+                      Label
+                      (name * (input + output))) :=
+  forall n,
+    ~ root n ->
+    In n (snd e.(evt_a)).(odnwNodes) ->
+    ~ In n failed ->
+    exists d,
+      (snd e.(evt_a)).(odnwState) n = Some d /\
+      aggregate d = 1%g.
+
+Lemma non_root_nodes_eventually_have_unit :
+  forall s failed,
+    event_step_star step_ordered_dynamic_failure step_ordered_dynamic_failure_init (hd s) ->
+    failed = fst (hd s).(evt_a) ->
+    lb_step_execution lb_step_ordered_dynamic_failure s ->
+    continuously (now (non_root_nodes_have_unit failed)) s.
+Proof.
+Admitted.
+
+Definition mass_conserved_opt_event
+           (failed : list name)
+           (e : event (list name * ordered_dynamic_network)
+                      Label
+                      (name * (input + output))) : Prop :=
+  let (failed, net) := e.(evt_a) in
+  conserves_network_mass_opt
+    (remove_all name_eq_dec failed net.(odnwNodes))
+    net.(odnwNodes) net.(odnwPackets) net.(odnwState).
+
+Lemma mass_always_conserved :
+  forall s failed,
+    event_step_star step_ordered_dynamic_failure step_ordered_dynamic_failure_init (hd s) ->
+    failed = fst (hd s).(evt_a) ->
+    lb_step_execution lb_step_ordered_dynamic_failure s ->
+    always (now (mass_conserved_opt_event failed)) s.
+Proof.
+Admitted.
+
+Definition no_fail_incoming_active_event
+           (failed : list name)
+           (e : event (list name * ordered_dynamic_network)
+                      Label
+                      (name * (input + output))) : Prop :=
+  forall src dst,
+    In dst e.(evt_a).(snd).(odnwNodes) ->
+    ~ In dst failed ->
+    ~ In Fail (e.(evt_a).(snd).(odnwPackets) src dst).
+
+Definition no_aggregate_incoming_active_event
+           (failed : list name)
+           (e : event (list name * ordered_dynamic_network)
+                      Label
+                      (name * (input + output))) : Prop :=
+  forall src dst,
+    In dst e.(evt_a).(snd).(odnwNodes) ->
+    ~ In dst failed ->
+    forall v,
+      ~ In (Aggregate v) (e.(evt_a).(snd).(odnwPackets) src dst).
+
+Lemma fail_msgs_stop :
+  forall failed s,
+    failed = (hd s).(evt_a).(fst) ->
+    event_step_star step_ordered_dynamic_failure step_ordered_dynamic_failure_init (hd s) ->
+    lb_step_execution lb_step_ordered_dynamic_failure s ->
+    continuously (now (no_fail_incoming_active_event failed)) s.
+Proof.
+Admitted.
+
+Definition correct_root_aggregate
+           (n : name)
+           (e : event (list name * ordered_dynamic_network)
+                      Label
+                      (name * (input + output))) : Prop :=
+  sum_local
+    (Nodes_data_opt
+       (remove_all name_eq_dec e.(evt_a).(fst) e.(evt_a).(snd).(odnwNodes))
+       e.(evt_a).(snd).(odnwState)) =
+  node_aggregate e.(evt_a).(snd).(odnwState) n.
+
+(* This lemma lets us prove stabilization once we prove that its hypotheses
+   about the network eventually hold. *)
+Lemma no_noise_means_correct_root_aggregate :
+  forall e n,
+    root n ->
+    In n e.(evt_a).(snd).(odnwNodes) ->
+    ~ In n e.(evt_a).(fst) ->
+    mass_conserved_opt_event e.(evt_a).(fst) e ->
+    no_fail_incoming_active_event e.(evt_a).(fst) e ->
+    no_aggregate_incoming_active_event e.(evt_a).(fst) e ->
+    non_root_nodes_have_unit e.(evt_a).(fst) e ->
+    correct_root_aggregate n e.
+Proof.
+  unfold mass_conserved_opt_event, conserves_network_mass_opt, correct_root_aggregate.
+  intros.
+  break_let; simpl in *.
+  remember (remove_all name_eq_dec l o.(odnwNodes)) as live_nodes.
+  assert (sum_fail_balance_incoming_active_opt o.(odnwNodes) live_nodes o.(odnwPackets) o.(odnwState) = 1%g).
+  {
+    unfold no_fail_incoming_active_event in *.
+    unfold sum_fail_balance_incoming_active_opt.
+    admit.
+  }
+  assert (sum_aggregate_msg_incoming_active o.(odnwNodes) live_nodes o.(odnwPackets) = 1%g).
+  {
+    unfold sum_aggregate_msg_incoming_active.
+    unfold sum_aggregate_msg_incoming.
+    unfold no_aggregate_incoming_active_event in *.
+    unfold sum_aggregate_msg.
+    unfold aggregate_sum_fold.
+    admit.
+  }
+  repeat find_rewrite.
+  gsimpl.
+Admitted.
+
+Theorem churn_free_stabilization :
   forall s, event_step_star step_ordered_dynamic_failure step_ordered_dynamic_failure_init (hd s) ->
        connected (hd s).(evt_a).(snd).(odnwNodes) ->
        lb_step_execution lb_step_ordered_dynamic_failure s ->
        weak_fairness lb_step_ordered_dynamic_failure Tau s ->
        forall n, root n -> In n (hd s).(evt_a).(snd).(odnwNodes) ->
-       eventually (always (now (fun e =>
-                                  sum_local 
-                                    (Nodes_data_opt 
-                                       (remove_all name_eq_dec e.(evt_a).(fst) e.(evt_a).(snd).(odnwNodes))
-                                       e.(evt_a).(snd).(odnwState)) =
-                                  node_aggregate e.(evt_a).(snd).(odnwState) n))) s.
+       continuously (now (correct_root_aggregate n)) s.
 Proof.
+  intros.
+  find_copy_eapply_lem_hyp fail_msgs_stop; eauto.
+  find_copy_eapply_lem_hyp non_root_nodes_eventually_have_unit; eauto.
+  pose proof (continuously_and_tl H5 H6).
 Admitted.
 
 End TreeAggregationCorrect.
